chore: Update for awslabs/smithy-dafny/pull/189 (#153)
Account for the changes in awslabs/smithy-dafny#189, mainly depending on the classpath for AWS traits instead of local copies, and using the aws.api#service$sdkId value to name Dafny clients when present instead of the shape name.

Regenerated all the Smithy-generated code and reviewed the diff, although I think there have been other smithy-dafny changes besides mine that haven't been applied, specifically around component ordering.

Also renamed KeyManagementService back to TrentService as it was in the original Smithy model, now that smithy-dafny uses the sdkId instead.

Co-authored-by: José Corella <39066999+josecorella@users.noreply.github.com>

AwsCryptographicMaterialProviders/runtimes/java/src/main/smithy-generated/software/amazon/cryptography/materialProviders/ClientSupplier.java
@@ -5,7 +5,7 @@ package software.amazon.cryptography.materialProviders;
 
 import Dafny.Aws.Cryptography.MaterialProviders.Types.Error;
 import Dafny.Com.Amazonaws.Kms.Shim;
-import Dafny.Com.Amazonaws.Kms.Types.IKeyManagementServiceClient;
+import Dafny.Com.Amazonaws.Kms.Types.IKMSClient;
 import Wrappers_Compile.Result;
 import java.lang.Exception;
 import java.lang.IllegalArgumentException;
@@ -43,11 +43,11 @@ public final class ClientSupplier implements IClientSupplier {
 
   public KmsClient GetClient(GetClientInput nativeValue) {
     Dafny.Aws.Cryptography.MaterialProviders.Types.GetClientInput dafnyValue = ToDafny.GetClientInput(nativeValue);
-    Result<IKeyManagementServiceClient, Error> result = this._impl.GetClient(dafnyValue);
+    Result<IKMSClient, Error> result = this._impl.GetClient(dafnyValue);
     if (result.is_Failure()) {
       throw ToNative.Error(result.dtor_error());
     }
-    return Dafny.Com.Amazonaws.Kms.ToNative.KeyManagementService(result.dtor_value());
+    return Dafny.Com.Amazonaws.Kms.ToNative.TrentService(result.dtor_value());
   }
 
   private static final class NativeWrapper implements Dafny.Aws.Cryptography.MaterialProviders.Types.IClientSupplier {
@@ -60,12 +60,12 @@ public final class ClientSupplier implements IClientSupplier {
       this._impl = nativeImpl;
     }
 
-    public Result<IKeyManagementServiceClient, Error> GetClient(
+    public Result<IKMSClient, Error> GetClient(
         Dafny.Aws.Cryptography.MaterialProviders.Types.GetClientInput dafnyInput) {
       GetClientInput nativeInput = ToNative.GetClientInput(dafnyInput);
       try {
         KmsClient nativeOutput = this._impl.GetClient(nativeInput);
-        IKeyManagementServiceClient dafnyOutput = new Shim(nativeOutput, null);
+        IKMSClient dafnyOutput = new Shim(nativeOutput, null);
         return Result.create_Success(dafnyOutput);
       } catch (NativeError ex) {
         return Result.create_Failure(ToDafny.Error(ex));
@@ -75,7 +75,7 @@ public final class ClientSupplier implements IClientSupplier {
       }
     }
 
-    public Result<IKeyManagementServiceClient, Error> GetClient_k(
+    public Result<IKMSClient, Error> GetClient_k(
         Dafny.Aws.Cryptography.MaterialProviders.Types.GetClientInput dafnyInput) {
       throw NativeError.builder().message("Not supported at this time.").build();
     }
