AwsCryptographicMaterialProviders/runtimes/net/Generated/ClientSupplierBase.cs
@@ -2,15 +2,12 @@
 // SPDX-License-Identifier: Apache-2.0
 // Do not modify this file. This file is machine generated, and any changes to it will be overwritten.
 using System;
-using AWS.Cryptography.MaterialProviders;
-namespace AWS.Cryptography.MaterialProviders
-{
-  public abstract class ClientSupplierBase : IClientSupplier
-  {
-    public Amazon.KeyManagementService.IAmazonKeyManagementService GetClient(AWS.Cryptography.MaterialProviders.GetClientInput input)
-    {
-      input.Validate(); return _GetClient(input);
-    }
-    protected abstract Amazon.KeyManagementService.IAmazonKeyManagementService _GetClient(AWS.Cryptography.MaterialProviders.GetClientInput input);
-  }
+ using AWS.Cryptography.MaterialProviders; namespace AWS.Cryptography.MaterialProviders {
+ public abstract class ClientSupplierBase : IClientSupplier {
+ public Amazon.KeyManagementService.IAmazonKeyManagementService GetClient ( AWS.Cryptography.MaterialProviders.GetClientInput input )
+ {
+ input.Validate(); return _GetClient ( input ) ;
+}
+ protected abstract Amazon.KeyManagementService.IAmazonKeyManagementService _GetClient ( AWS.Cryptography.MaterialProviders.GetClientInput input ) ;
+}
 }
