AwsCryptographicMaterialProviders/runtimes/net/Generated/CollectionOfErrors.cs
@@ -2,14 +2,11 @@
 // SPDX-License-Identifier: Apache-2.0
 // Do not modify this file. This file is machine generated, and any changes to it will be overwritten.
 using System;
-using AWS.Cryptography.MaterialProviders;
-namespace AWS.Cryptography.MaterialProviders
-{
-  public class CollectionOfErrors : Exception
-  {
-    public readonly System.Collections.Generic.List<Exception> list;
-    public CollectionOfErrors(System.Collections.Generic.List<Exception> list) : base("CollectionOfErrors") { this.list = list; }
-    public CollectionOfErrors() : base("CollectionOfErrors") { this.list = new System.Collections.Generic.List<Exception>(); }
-  }
+ using AWS.Cryptography.MaterialProviders; namespace AWS.Cryptography.MaterialProviders {
+ public class CollectionOfErrors : Exception {
+  public readonly System.Collections.Generic.List<Exception> list;
+  public CollectionOfErrors(System.Collections.Generic.List<Exception> list) : base("CollectionOfErrors") { this.list = list; }
+  public CollectionOfErrors() : base("CollectionOfErrors") { this.list = new System.Collections.Generic.List<Exception>(); }
+}
 
 }
