AwsCryptographicMaterialProviders/runtimes/net/Generated/CryptographicMaterialsManager.cs
@@ -2,29 +2,24 @@
 // SPDX-License-Identifier: Apache-2.0
 // Do not modify this file. This file is machine generated, and any changes to it will be overwritten.
 using System;
-using System.IO;
-using System.Collections.Generic;
-using AWS.Cryptography.MaterialProviders;
-using Dafny.Aws.Cryptography.MaterialProviders.Types;
-namespace AWS.Cryptography.MaterialProviders
-{
-  internal class CryptographicMaterialsManager : CryptographicMaterialsManagerBase
-  {
-    internal readonly Dafny.Aws.Cryptography.MaterialProviders.Types.ICryptographicMaterialsManager _impl;
-    internal CryptographicMaterialsManager(Dafny.Aws.Cryptography.MaterialProviders.Types.ICryptographicMaterialsManager impl) { this._impl = impl; }
-    protected override AWS.Cryptography.MaterialProviders.GetEncryptionMaterialsOutput _GetEncryptionMaterials(AWS.Cryptography.MaterialProviders.GetEncryptionMaterialsInput input)
-    {
-      Dafny.Aws.Cryptography.MaterialProviders.Types._IGetEncryptionMaterialsInput internalInput = TypeConversion.ToDafny_N3_aws__N12_cryptography__N17_materialProviders__S27_GetEncryptionMaterialsInput(input);
-      Wrappers_Compile._IResult<Dafny.Aws.Cryptography.MaterialProviders.Types._IGetEncryptionMaterialsOutput, Dafny.Aws.Cryptography.MaterialProviders.Types._IError> result = this._impl.GetEncryptionMaterials(internalInput);
-      if (result.is_Failure) throw TypeConversion.FromDafny_CommonError(result.dtor_error);
-      return TypeConversion.FromDafny_N3_aws__N12_cryptography__N17_materialProviders__S28_GetEncryptionMaterialsOutput(result.dtor_value);
-    }
-    protected override AWS.Cryptography.MaterialProviders.DecryptMaterialsOutput _DecryptMaterials(AWS.Cryptography.MaterialProviders.DecryptMaterialsInput input)
-    {
-      Dafny.Aws.Cryptography.MaterialProviders.Types._IDecryptMaterialsInput internalInput = TypeConversion.ToDafny_N3_aws__N12_cryptography__N17_materialProviders__S21_DecryptMaterialsInput(input);
-      Wrappers_Compile._IResult<Dafny.Aws.Cryptography.MaterialProviders.Types._IDecryptMaterialsOutput, Dafny.Aws.Cryptography.MaterialProviders.Types._IError> result = this._impl.DecryptMaterials(internalInput);
-      if (result.is_Failure) throw TypeConversion.FromDafny_CommonError(result.dtor_error);
-      return TypeConversion.FromDafny_N3_aws__N12_cryptography__N17_materialProviders__S22_DecryptMaterialsOutput(result.dtor_value);
-    }
-  }
+ using System.IO;
+ using System.Collections.Generic;
+ using AWS.Cryptography.MaterialProviders;
+ using Dafny.Aws.Cryptography.MaterialProviders.Types; namespace AWS.Cryptography.MaterialProviders {
+ internal class CryptographicMaterialsManager : CryptographicMaterialsManagerBase {
+ internal readonly Dafny.Aws.Cryptography.MaterialProviders.Types.ICryptographicMaterialsManager _impl;
+ internal CryptographicMaterialsManager(Dafny.Aws.Cryptography.MaterialProviders.Types.ICryptographicMaterialsManager impl) { this._impl = impl; }
+ protected override AWS.Cryptography.MaterialProviders.GetEncryptionMaterialsOutput _GetEncryptionMaterials(AWS.Cryptography.MaterialProviders.GetEncryptionMaterialsInput input) {
+ Dafny.Aws.Cryptography.MaterialProviders.Types._IGetEncryptionMaterialsInput internalInput = TypeConversion.ToDafny_N3_aws__N12_cryptography__N17_materialProviders__S27_GetEncryptionMaterialsInput(input);
+ Wrappers_Compile._IResult<Dafny.Aws.Cryptography.MaterialProviders.Types._IGetEncryptionMaterialsOutput, Dafny.Aws.Cryptography.MaterialProviders.Types._IError> result = this._impl.GetEncryptionMaterials(internalInput);
+ if (result.is_Failure) throw TypeConversion.FromDafny_CommonError(result.dtor_error);
+ return TypeConversion.FromDafny_N3_aws__N12_cryptography__N17_materialProviders__S28_GetEncryptionMaterialsOutput(result.dtor_value);
+}
+ protected override AWS.Cryptography.MaterialProviders.DecryptMaterialsOutput _DecryptMaterials(AWS.Cryptography.MaterialProviders.DecryptMaterialsInput input) {
+ Dafny.Aws.Cryptography.MaterialProviders.Types._IDecryptMaterialsInput internalInput = TypeConversion.ToDafny_N3_aws__N12_cryptography__N17_materialProviders__S21_DecryptMaterialsInput(input);
+ Wrappers_Compile._IResult<Dafny.Aws.Cryptography.MaterialProviders.Types._IDecryptMaterialsOutput, Dafny.Aws.Cryptography.MaterialProviders.Types._IError> result = this._impl.DecryptMaterials(internalInput);
+ if (result.is_Failure) throw TypeConversion.FromDafny_CommonError(result.dtor_error);
+ return TypeConversion.FromDafny_N3_aws__N12_cryptography__N17_materialProviders__S22_DecryptMaterialsOutput(result.dtor_value);
+}
+}
 }
