AwsCryptographicMaterialProviders/runtimes/net/Generated/DeleteCacheEntryInput.cs
@@ -2,25 +2,19 @@
 // SPDX-License-Identifier: Apache-2.0
 // Do not modify this file. This file is machine generated, and any changes to it will be overwritten.
 using System;
-using AWS.Cryptography.MaterialProviders;
-namespace AWS.Cryptography.MaterialProviders
-{
-  public class DeleteCacheEntryInput
-  {
-    private System.IO.MemoryStream _identifier;
-    public System.IO.MemoryStream Identifier
-    {
-      get { return this._identifier; }
-      set { this._identifier = value; }
-    }
-    public bool IsSetIdentifier()
-    {
-      return this._identifier != null;
-    }
-    public void Validate()
-    {
-      if (!IsSetIdentifier()) throw new System.ArgumentException("Missing value for required property 'Identifier'");
+ using AWS.Cryptography.MaterialProviders; namespace AWS.Cryptography.MaterialProviders {
+ public class DeleteCacheEntryInput {
+ private System.IO.MemoryStream _identifier ;
+ public System.IO.MemoryStream Identifier {
+ get { return this._identifier; }
+ set { this._identifier = value; }
+}
+ public bool IsSetIdentifier () {
+ return this._identifier != null;
+}
+ public void Validate() {
+ if (!IsSetIdentifier()) throw new System.ArgumentException("Missing value for required property 'Identifier'");
 
-    }
-  }
+}
+}
 }
