AwsCryptographicMaterialProviders/runtimes/net/Generated/GetBranchKeyIdInput.cs
@@ -2,25 +2,19 @@
 // SPDX-License-Identifier: Apache-2.0
 // Do not modify this file. This file is machine generated, and any changes to it will be overwritten.
 using System;
-using AWS.Cryptography.MaterialProviders;
-namespace AWS.Cryptography.MaterialProviders
-{
-  public class GetBranchKeyIdInput
-  {
-    private System.Collections.Generic.Dictionary<string, string> _encryptionContext;
-    public System.Collections.Generic.Dictionary<string, string> EncryptionContext
-    {
-      get { return this._encryptionContext; }
-      set { this._encryptionContext = value; }
-    }
-    public bool IsSetEncryptionContext()
-    {
-      return this._encryptionContext != null;
-    }
-    public void Validate()
-    {
-      if (!IsSetEncryptionContext()) throw new System.ArgumentException("Missing value for required property 'EncryptionContext'");
+ using AWS.Cryptography.MaterialProviders; namespace AWS.Cryptography.MaterialProviders {
+ public class GetBranchKeyIdInput {
+ private System.Collections.Generic.Dictionary<string, string> _encryptionContext ;
+ public System.Collections.Generic.Dictionary<string, string> EncryptionContext {
+ get { return this._encryptionContext; }
+ set { this._encryptionContext = value; }
+}
+ public bool IsSetEncryptionContext () {
+ return this._encryptionContext != null;
+}
+ public void Validate() {
+ if (!IsSetEncryptionContext()) throw new System.ArgumentException("Missing value for required property 'EncryptionContext'");
 
-    }
-  }
+}
+}
 }
