AwsCryptographicMaterialProviders/runtimes/net/Generated/IBranchKeyIdSupplier.cs
@@ -2,11 +2,8 @@
 // SPDX-License-Identifier: Apache-2.0
 // Do not modify this file. This file is machine generated, and any changes to it will be overwritten.
 using System;
-using AWS.Cryptography.MaterialProviders;
-namespace AWS.Cryptography.MaterialProviders
-{
-  public interface IBranchKeyIdSupplier
-  {
-    AWS.Cryptography.MaterialProviders.GetBranchKeyIdOutput GetBranchKeyId(AWS.Cryptography.MaterialProviders.GetBranchKeyIdInput input);
-  }
+ using AWS.Cryptography.MaterialProviders; namespace AWS.Cryptography.MaterialProviders {
+ public interface IBranchKeyIdSupplier {
+ AWS.Cryptography.MaterialProviders.GetBranchKeyIdOutput GetBranchKeyId ( AWS.Cryptography.MaterialProviders.GetBranchKeyIdInput input ) ;
+}
 }
