AwsCryptographicMaterialProviders/runtimes/net/Generated/ICryptographicMaterialsCache.cs
@@ -2,14 +2,11 @@
 // SPDX-License-Identifier: Apache-2.0
 // Do not modify this file. This file is machine generated, and any changes to it will be overwritten.
 using System;
-using AWS.Cryptography.MaterialProviders;
-namespace AWS.Cryptography.MaterialProviders
-{
-  public interface ICryptographicMaterialsCache
-  {
-    void PutCacheEntry(AWS.Cryptography.MaterialProviders.PutCacheEntryInput input);
-    AWS.Cryptography.MaterialProviders.GetCacheEntryOutput GetCacheEntry(AWS.Cryptography.MaterialProviders.GetCacheEntryInput input);
-    void UpdaterUsageMetadata(AWS.Cryptography.MaterialProviders.UpdaterUsageMetadataInput input);
-    void DeleteCacheEntry(AWS.Cryptography.MaterialProviders.DeleteCacheEntryInput input);
-  }
+ using AWS.Cryptography.MaterialProviders; namespace AWS.Cryptography.MaterialProviders {
+ public interface ICryptographicMaterialsCache {
+ void PutCacheEntry ( AWS.Cryptography.MaterialProviders.PutCacheEntryInput input ) ;
+ AWS.Cryptography.MaterialProviders.GetCacheEntryOutput GetCacheEntry ( AWS.Cryptography.MaterialProviders.GetCacheEntryInput input ) ;
+ void UpdaterUsageMetadata ( AWS.Cryptography.MaterialProviders.UpdaterUsageMetadataInput input ) ;
+ void DeleteCacheEntry ( AWS.Cryptography.MaterialProviders.DeleteCacheEntryInput input ) ;
+}
 }
