AwsCryptographicMaterialProviders/runtimes/net/Generated/Materials.cs
@@ -2,50 +2,40 @@
 // SPDX-License-Identifier: Apache-2.0
 // Do not modify this file. This file is machine generated, and any changes to it will be overwritten.
 using System;
-using AWS.Cryptography.MaterialProviders;
-namespace AWS.Cryptography.MaterialProviders
-{
-  public class Materials
-  {
-    private AWS.Cryptography.MaterialProviders.EncryptionMaterials _encryption;
-    private AWS.Cryptography.MaterialProviders.DecryptionMaterials _decryption;
-    private AWS.Cryptography.MaterialProviders.HierarchicalMaterials _hierarchical;
-    public AWS.Cryptography.MaterialProviders.EncryptionMaterials Encryption
-    {
-      get { return this._encryption; }
-      set { this._encryption = value; }
-    }
-    public bool IsSetEncryption()
-    {
-      return this._encryption != null;
-    }
-    public AWS.Cryptography.MaterialProviders.DecryptionMaterials Decryption
-    {
-      get { return this._decryption; }
-      set { this._decryption = value; }
-    }
-    public bool IsSetDecryption()
-    {
-      return this._decryption != null;
-    }
-    public AWS.Cryptography.MaterialProviders.HierarchicalMaterials Hierarchical
-    {
-      get { return this._hierarchical; }
-      set { this._hierarchical = value; }
-    }
-    public bool IsSetHierarchical()
-    {
-      return this._hierarchical != null;
-    }
-    public void Validate()
-    {
-      var numberOfPropertiesSet = Convert.ToUInt16(IsSetEncryption()) +
-      Convert.ToUInt16(IsSetDecryption()) +
-      Convert.ToUInt16(IsSetHierarchical());
-      if (numberOfPropertiesSet == 0) throw new System.ArgumentException("No union value set");
+ using AWS.Cryptography.MaterialProviders; namespace AWS.Cryptography.MaterialProviders {
+ public class Materials {
+ private AWS.Cryptography.MaterialProviders.EncryptionMaterials _encryption ;
+ private AWS.Cryptography.MaterialProviders.DecryptionMaterials _decryption ;
+ private AWS.Cryptography.MaterialProviders.HierarchicalMaterials _hierarchical ;
+ public AWS.Cryptography.MaterialProviders.EncryptionMaterials Encryption {
+ get { return this._encryption; }
+ set { this._encryption = value; }
+}
+ public bool IsSetEncryption () {
+ return this._encryption != null;
+}
+ public AWS.Cryptography.MaterialProviders.DecryptionMaterials Decryption {
+ get { return this._decryption; }
+ set { this._decryption = value; }
+}
+ public bool IsSetDecryption () {
+ return this._decryption != null;
+}
+ public AWS.Cryptography.MaterialProviders.HierarchicalMaterials Hierarchical {
+ get { return this._hierarchical; }
+ set { this._hierarchical = value; }
+}
+ public bool IsSetHierarchical () {
+ return this._hierarchical != null;
+}
+ public void Validate() {
+ var numberOfPropertiesSet = Convert.ToUInt16(IsSetEncryption()) +
+ Convert.ToUInt16(IsSetDecryption()) +
+ Convert.ToUInt16(IsSetHierarchical()) ;
+ if (numberOfPropertiesSet == 0) throw new System.ArgumentException("No union value set");
 
-      if (numberOfPropertiesSet > 1) throw new System.ArgumentException("Multiple union values set");
+ if (numberOfPropertiesSet > 1) throw new System.ArgumentException("Multiple union values set");
 
-    }
-  }
+}
+}
 }
