ComAmazonawsKms/runtimes/net/Extern/KMSClient.cs
@@ -13,7 +13,7 @@ namespace Dafny.Com.Amazonaws.Kms
     
     public static
       _IResult<
-        Types.IKeyManagementServiceClient,
+        Types.IKMSClient,
         Types._IError
       >
       KMSClient()
@@ -23,14 +23,14 @@ namespace Dafny.Com.Amazonaws.Kms
       var client = new AmazonKeyManagementServiceClient();
 
       return Result<
-        Types.IKeyManagementServiceClient,
+        Types.IKMSClient,
         Types._IError
       >
         .create_Success(new KeyManagementServiceShim(client));
     }
 
         public static _IOption<bool> RegionMatch(
-            Dafny.Com.Amazonaws.Kms.Types.IKeyManagementServiceClient client,
+            Dafny.Com.Amazonaws.Kms.Types.IKMSClient client,
             Dafny.ISequence<char> region)
         {
             string regionStr = TypeConversion.FromDafny_N6_smithy__N3_api__S6_String(region);
